Proof case Jnz FTLR

theories/ftlr/Jnz.v
@@ -1,9 +1,9 @@
-From cap_machine Require Export logrel.
 From iris.proofmode Require Import proofmode.
 From iris.program_logic Require Import weakestpre adequacy lifting.
 From stdpp Require Import base.
+From cap_machine Require Export logrel register_tactics.
 From cap_machine.ftlr Require Import ftlr_base.
-From cap_machine.rules Require Import rules_base rules_Jnz.
+From cap_machine.rules Require Import rules_Jnz.
 
 Section fundamental.
   Context {Σ:gFunctors} {memg:memG Σ} {regg:regG Σ} {sealsg: sealStoreG Σ}
@@ -15,80 +15,740 @@ Section fundamental.
   Implicit Types w : (leibnizO Word).
   Implicit Types interp : (D).
 
-  Lemma jnz_case (r : leibnizO Reg) (p : Perm)
-        (b e a : Addr) (w : Word) (r1 r2 : RegName) (P : D):
-    ftlr_instr r p b e a w (Jnz r1 r2) P.
+
+  (* TODO the whole proof strategy is very similar to the one for Jmp.
+     Is there a way to factor out both of them ? *)
+
+  (* Mask after the jump, depending on the address of the pc and the address
+   of a *)
+  Definition allow_jnz_mask (pc_a a : Addr) : coPset
+    :=
+    if decide (pc_a = a)
+    then (⊤ ∖ ↑logN.@pc_a ∖ ↑logN.@(a^+1)%a)
+    else
+      if decide (pc_a = (a^+1)%a)
+      then (⊤ ∖ ↑logN.@pc_a ∖ ↑logN.@a)
+      else (⊤ ∖ ↑logN.@pc_a ∖ ↑logN.@a ∖ ↑logN.@(a^+1)%a).
+
+
+  Definition allow_jnz_mask_reg (regs : Reg) (dst src : RegName)
+    (pc_a : Addr) (p : Perm) (b e a : Addr) (wsrc : Word)
+    : coPset :=
+    if decide (reg_allows_IE_jmp regs dst p b e a
+               /\ regs !! src = Some wsrc
+               /\ nonZero wsrc = true)
+    then allow_jnz_mask pc_a a
+    else (⊤ ∖ ↑logN.@pc_a).
+
+  (* The necessary resources to close the region again,
+     except for the points to predicate, which we will store separately *)
+  Definition region_open_resources2
+    (pc_a : Addr) (a : Addr)
+    (w1 : Word) (w2 : Word)
+    (P1 P2 : D)
+    : iProp Σ :=
+    ▷ P1 w1 ∗ ▷ P2 w2
+       ∗ persistent_cond P1 ∗ persistent_cond P2
+       ∗ ((▷ ∃ w1 w2, a ↦ₐ w1 ∗ P1 w1 ∗ (a^+1)%a ↦ₐ w2 ∗ P2 w2)
+          ={allow_jnz_mask pc_a a, ⊤ ∖ ↑logN.@pc_a}=∗ emp)%I.
+
+  Definition region_open_resources
+    (pc_a : Addr) (a : Addr) (w : Word)
+    (P : D)
+    : iProp Σ :=
+    (▷ P w
+       ∗ persistent_cond P
+       ∗ ((▷ ∃ w, a ↦ₐ w ∗ P w)
+        ={allow_jnz_mask pc_a a, ⊤ ∖ ↑logN.@pc_a}=∗ emp))%I.
+
+  Definition region_open_resources'
+    (pc_a : Addr) (a : Addr) (w' : Word)
+    (P : D)
+    : iProp Σ :=
+    (▷ P w'
+       ∗ persistent_cond P
+       ∗ ((▷ ∃ w', (a^+1)%a ↦ₐ w' ∗ P w')
+        ={allow_jnz_mask pc_a a, ⊤ ∖ ↑logN.@pc_a}=∗ emp))%I.
+
+  (* Description of what the resources are supposed to look like after opening the
+     region if we need to, but before closing the region up again*)
+  Definition allow_jnz_res (regs : Reg) (dst src : RegName)
+    (pc_a : Addr) (p : Perm) (b e a : Addr) (wsrc : Word)
+    (P1 P2 : D): iProp Σ :=
+    ( ⌜read_reg_inr regs dst p b e a⌝ ∗
+      ⌜regs !! src = Some wsrc⌝ ∗
+       if decide (reg_allows_IE_jmp regs dst p b e a
+               /\ regs !! src = Some wsrc
+               /\ nonZero wsrc = true)
+       then
+         (∀ w1 w2 regs', ▷ □ (P1 w1 ∗ (P2 w2 ∨ ⌜ is_int w2 ⌝)
+                              -∗ (interp_expr_gen interp regs' w1 w2)))
+           ∗
+           |={⊤ ∖ ↑logN.@pc_a, allow_jnz_mask pc_a a}=>
+           (if decide (pc_a = a)
+            then ∃ w2, (a^+1)%a ↦ₐ w2 ∗ region_open_resources' pc_a a w2 P2
+            else
+              if decide (pc_a = (a^+1)%a)
+              then ∃ w1, a ↦ₐ w1 ∗ region_open_resources pc_a a w1 P1
+              else ∃ w1 w2, a ↦ₐ w1 ∗ (a^+1)%a ↦ₐ w2 ∗ region_open_resources2 pc_a a w1 w2 P1 P2
+           )
+       else True)%I.
+
+  Lemma create_jnz_res:
+    ∀ (regs : leibnizO Reg) (dst src : RegName)
+      (pc_p : Perm) (pc_b pc_e pc_a : Addr)
+      (widc : Word)
+      (p : Perm) (b e a : Addr) (wsrc : Word),
+      pc_p <> IE ->
+      read_reg_inr (<[PC:=WCap pc_p pc_b pc_e pc_a]> (<[idc:= widc]> regs)) dst p b e a ->
+      (<[PC:=WCap pc_p pc_b pc_e pc_a]> (<[idc:= widc]> regs)) !! src = Some wsrc ->
+      (∀ (r' : RegName) (w : Word), ⌜r' ≠ PC⌝ → ⌜r' ≠ idc⌝ → ⌜regs !! r' = Some w⌝ → (fixpoint interp1) w)
+      -∗ interp widc
+      -∗ ∃ (P1 P2 : D),
+           allow_jnz_res (<[PC:=WCap pc_p pc_b pc_e pc_a]> (<[idc:=widc]> regs)) dst src pc_a p b
+             e a wsrc P1 P2.
+  Proof.
+    intros regs dst src pc_p pc_b pc_e pc_a widc p b e a wsrc Hpc_p HVr Hsrc.
+    iIntros "#Hreg #Hwidc".
+    iFrame "%".
+    case_decide as Hallows; cycle 1.
+    - by iExists (λne _, True%I), (λne _, True%I).
+    - rewrite /allow_jnz_mask.
+      destruct Hallows as ((Hreg & -> & Hwb & Hwb') & Hsrc' & Hnz).
+      assert (a <> (a^+1)%a) by (apply andb_prop in Hwb as [_ Hge]; solve_addr).
+      apply Is_true_true_2 in Hwb, Hwb'.
+      assert ( withinBounds b e a /\ withinBounds b e (a^+1)%a) as Hwbs by auto.
+
+      assert (dst ≠ PC) as Hneq by (destruct (decide (dst = PC)) ; simplify_map_eq; auto).
+      rewrite lookup_insert_ne //= in Hreg.
+
+      (* TODO there are plenty of similar case, find a way to factor out *)
+
+      case_decide as Ha; simplify_eq.
+      {
+        destruct (decide (dst = idc)) as [|Hneq']; simplify_map_eq.
+        + rewrite fixpoint_interp1_eq /=.
+          iDestruct ("Hwidc" $! Hwbs) as (P1 P2) "(Hpers_P1 & Hpers_P2 & Hinv_a & Hinv_a' & Hexec)".
+          iExists P1, P2.
+          iFrame "#".
+          iMod (inv_acc (⊤ ∖ ↑logN.@a) with "Hinv_a'") as "[Hrefinv_a' Hcls_a']";[solve_ndisj|].
+          iDestruct "Hrefinv_a'" as (w2) "[>Ha' HPa']".
+          iExists w2.
+          iFrame "∗ #".
+          rewrite /allow_jnz_mask. do 2 (case_decide ; solve_addr).
+        + iDestruct ("Hreg" $! dst _ Hneq Hneq' Hreg) as "Hvsrc".
+          rewrite (fixpoint_interp1_eq (WCap _ _ _ _)) /=.
+          iDestruct ("Hvsrc" $! Hwbs) as (P1 P2) "(Hpers_P1 & Hpers_P2 & Hinv_a & Hinv_a' & Hexec)".
+          iExists P1, P2.
+          iFrame "#".
+          iMod (inv_acc (⊤ ∖ ↑logN.@a) with "Hinv_a'") as "[Hrefinv_a' Hcls_a']";[solve_ndisj|].
+          iDestruct "Hrefinv_a'" as (w2) "[>Ha' HPa']".
+          iExists w2.
+          iFrame "∗ #".
+          rewrite /allow_jnz_mask. do 2 (case_decide ; solve_addr).
+      }
+
+      case_decide as Ha'; simplify_eq.
+      {
+        destruct (decide (dst = idc)) as [|Hneq']; simplify_map_eq.
+        + rewrite fixpoint_interp1_eq /=.
+          iDestruct ("Hwidc" $! Hwbs) as (P1 P2) "(Hpers_P1 & Hpers_P2 & Hinv_a & Hinv_a' & Hexec)".
+          iExists P1, P2.
+          iFrame "#".
+          iMod (inv_acc (⊤ ∖ ↑logN.@(a ^+ 1)%a) with "Hinv_a") as "[Hrefinv_a Hcls_a]";[solve_ndisj|].
+          iDestruct "Hrefinv_a" as (w1) "[>Ha HPa]".
+          iExists w1.
+          iFrame "∗ #".
+          rewrite /allow_jnz_mask. do 2 (case_decide ; try solve_addr).
+        + iDestruct ("Hreg" $! dst _ Hneq Hneq' Hreg) as "Hvsrc".
+          rewrite (fixpoint_interp1_eq (WCap _ _ _ _)) /=.
+          iDestruct ("Hvsrc" $! Hwbs) as (P1 P2) "(Hpers_P1 & Hpers_P2 & Hinv_a & Hinv_a' & Hexec)".
+          iExists P1, P2.
+          iFrame "#".
+          iMod (inv_acc (⊤ ∖ ↑logN.@(a ^+ 1)%a) with "Hinv_a") as "[Hrefinv_a Hcls_a]";[solve_ndisj|].
+          iDestruct "Hrefinv_a" as (w1) "[>Ha HPa]".
+          iExists w1.
+          iFrame "∗ #".
+          rewrite /allow_jnz_mask. do 2 (case_decide ; try solve_addr).
+      }
+
+      destruct (decide (dst = idc)) as [|Hneq']; simplify_map_eq.
+      + rewrite fixpoint_interp1_eq /=.
+        iDestruct ("Hwidc" $! Hwbs) as (P1 P2) "(Hpers_P1 & Hpers_P2 & Hinv_a & Hinv_a' & Hexec)".
+        iExists P1, P2.
+
+        iFrame "#".
+        iMod (inv_acc (⊤ ∖ ↑logN.@pc_a) with "Hinv_a") as "[Hrefinv_a Hcls_a]";[solve_ndisj|].
+        iMod (inv_acc (⊤ ∖ ↑logN.@pc_a ∖ ↑logN.@a) with "Hinv_a'") as "[Hrefinv_a' Hcls_a']";[solve_ndisj|].
+        iDestruct "Hrefinv_a" as (w1) "[>Ha HPa]".
+        iDestruct "Hrefinv_a'" as (w2) "[>Ha' HPa']".
+        iExists w1, w2.
+
+        iFrame "∗ #".
+        rewrite /region_open_resources2.
+        iModIntro.
+        iIntros "Ha".
+        iDestruct "Ha" as (w1' w2') "(Hw1' & HP1' & Hw2' & HP2')".
+        rewrite /allow_jnz_mask.
+        case_decide; simplify_eq.
+        case_decide; simplify_eq.
+        iMod ("Hcls_a'" with "[Hw2' HP2']") as "_"; first (iExists _ ; iFrame).
+        iMod ("Hcls_a" with "[Hw1' HP1']") as "_"; first (iExists _ ; iFrame).
+        done.
+      + iDestruct ("Hreg" $! dst _ Hneq Hneq' Hreg) as "Hvsrc".
+        rewrite (fixpoint_interp1_eq (WCap _ _ _ _)) /=.
+        iDestruct ("Hvsrc" $! Hwbs) as (P1 P2) "(Hpers_P1 & Hpers_P2 & Hinv_a & Hinv_a' & Hexec)".
+        iExists P1, P2.
+
+        iFrame "#".
+        iMod (inv_acc (⊤ ∖ ↑logN.@pc_a) with "Hinv_a") as "[Hrefinv_a Hcls_a]";[solve_ndisj|].
+        iMod (inv_acc (⊤ ∖ ↑logN.@pc_a ∖ ↑logN.@a) with "Hinv_a'") as "[Hrefinv_a' Hcls_a']";[solve_ndisj|].
+        iDestruct "Hrefinv_a" as (w1) "[>Ha HPa]".
+        iDestruct "Hrefinv_a'" as (w2) "[>Ha' HPa']".
+        iExists w1, w2.
+
+        iFrame "∗ #".
+        rewrite /region_open_resources2.
+        iModIntro.
+        iIntros "Ha".
+        iDestruct "Ha" as (w1' w2') "(Hw1' & HP1' & Hw2' & HP2')".
+        rewrite /allow_jnz_mask.
+        case_decide; simplify_eq.
+        case_decide; simplify_eq.
+        iMod ("Hcls_a'" with "[Hw2' HP2']") as "_"; first (iExists _ ; iFrame).
+        iMod ("Hcls_a" with "[Hw1' HP1']") as "_"; first (iExists _ ; iFrame).
+        done.
+  Qed.
+
+  Definition allow_jnz_mem
+    (regs : Reg) (mem : Mem) (dst src : RegName)
+    (pc_a : Addr) (pc_w : Word)
+    (p : Perm) (b e a : Addr) (wsrc : Word)
+    (P1 P2 : D) :=
+    ( ⌜read_reg_inr regs dst p b e a⌝ ∗
+      ⌜regs !! src = Some wsrc⌝ ∗
+       if decide (reg_allows_IE_jmp regs dst p b e a
+               /\ regs !! src = Some wsrc
+               /\ nonZero wsrc = true)
+       then (if decide (pc_a = a)
+             then ∃ w2, ⌜mem = <[(a^+1)%a:=w2]> (<[pc_a:=pc_w]> ∅)⌝ ∗ region_open_resources' pc_a a w2 P2
+             else
+               if decide (pc_a = (a^+1)%a)
+               then ∃ w1, ⌜mem = <[a:=w1]> (<[pc_a:=pc_w]> ∅)⌝ ∗ region_open_resources pc_a a w1 P1
+               else ∃ w1 w2,
+                   ⌜mem = <[(a^+1)%a:=w2]> (<[a:=w1]> (<[pc_a:=pc_w]> ∅))⌝
+                                             ∗ region_open_resources2 pc_a a w1 w2 P1 P2)
+       else ⌜mem = <[pc_a:=pc_w]> ∅⌝)%I.
+
+  Lemma jnz_res_implies_mem_map:
+    ∀ (regs : leibnizO Reg) (dst src: RegName)
+      (pc_a : Addr) (pc_w : Word)
+      (p : Perm) (b e a: Addr) (wsrc : Word)
+      (P1 P2:D),
+      allow_jnz_res regs dst src pc_a p b e a wsrc P1 P2
+      -∗ pc_a ↦ₐ pc_w
+      ={⊤ ∖ ↑logN.@pc_a, allow_jnz_mask_reg regs dst src pc_a p b e a wsrc}=∗
+      ∃ mem : Mem,
+          allow_jnz_mem regs mem dst src pc_a pc_w p b e a wsrc P1 P2
+            ∗ ▷ ([∗ map] a0↦w ∈ mem, a0 ↦ₐ w).
+  Proof.
+    intros regs dst src pc_a pc_w p b e a wsrc P1 P2.
+    iIntros "HJmpRes Hpc_a".
+    iDestruct "HJmpRes" as "(%Hrinr & %Hsrc & HJmpRes)".
+    rewrite /allow_jnz_mask /allow_jnz_mask_reg.
+
+    case_decide as Hdec ; cycle 1.
+    { rewrite /read_reg_inr in Hrinr.
+      iExists _.
+      iSplitL "HJmpRes".
+      + iModIntro. rewrite /allow_jnz_mem.
+        do 2 (iSplitR; auto).
+        case_decide; auto; first by exfalso.
+      + iModIntro. iNext. by iApply memMap_resource_1.
+    }
+    destruct Hdec as ((Hreg & -> & Hwb & Hwb') & Hsrc' & Hnz).
+    assert (a <> (a^+1)%a) as Haeq by (apply andb_prop in Hwb as [_ Hge]; solve_addr).
+    rewrite /allow_jnz_mask.
+    iDestruct "HJmpRes" as "[Hexec HJmpRes]".
+    iMod "HJmpRes" as "HJmpRes".
+
+    case_decide as Ha ; simplify_eq.
+    { (* pc_a = a *)
+      iDestruct "HJmpRes" as (w2) "[Ha' HJmpRest]".
+      iExists _.
+      iSplitL "HJmpRest".
+      + iSplitR; first auto.
+
+        case_decide as Hdec1.
+        2: {
+          apply not_and_r in Hdec1 as [Hcontra|Hcontra]; simplify_eq.
+          all: exfalso; apply Hcontra ; repeat (split ; auto).
+        }
+        case_decide; simplify_eq; auto.
+      + iModIntro. iNext.
+        rewrite memMap_resource_2ne; auto; iFrame.
+    }
+    (* pc_a ≠ a *)
+    case_decide as Ha' ; simplify_eq.
+    { (* pc_a = a+1 *)
+      iDestruct "HJmpRes" as (w1) "[Ha HJmpRest]".
+      iExists _.
+      iSplitL "HJmpRest".
+      + iSplitR; first auto.
+        case_decide as Hdec1.
+        2: {
+          apply not_and_r in Hdec1 as [Hcontra|Hcontra]; simplify_eq.
+          all: exfalso; apply Hcontra ; repeat (split ; auto).
+        }
+        case_decide; simplify_eq; auto.
+        case_decide; simplify_eq; auto.
+      + iModIntro. iNext.
+        rewrite memMap_resource_2ne; auto; iFrame.
+    }
+    (* pc_a ≠ a+1 *)
+
+    iDestruct "HJmpRes" as (w1 w2) "(Ha & Ha' & HJmpRest)".
+    iExists _.
+    iSplitL "HJmpRest".
+    + iSplitR; first auto.
+      case_decide as Hdec1.
+      2: {
+        apply not_and_r in Hdec1 as [Hcontra|Hcontra]; simplify_eq.
+        all: exfalso; apply Hcontra ; repeat (split ; auto).
+      }
+      case_decide; simplify_eq; auto.
+      case_decide; simplify_eq; auto.
+      iModIntro; auto.
+    + iModIntro. iNext.
+      rewrite memMap_resource_3ne; auto; iFrame.
+  Qed.
+
+  Lemma mem_map_implies_pure_conds:
+    ∀ (regs : leibnizO Reg) (mem : Mem) (dst src : RegName)
+      (pc_a : Addr) (pc_w : Word)
+      (p : Perm) (b e a : Addr) (wsrc : Word)
+      (P1 P2 : D),
+      allow_jnz_mem regs mem dst src pc_a pc_w p b e a wsrc P1 P2
+        -∗ ⌜mem !! pc_a = Some pc_w⌝
+          ∗ ⌜allow_jnz_mmap_or_true dst src regs mem⌝.
+  Proof.
+    iIntros (regs mem dst src pc_a pc_w p b e a wsrc P1 P2) "HJmpMem".
+    iDestruct "HJmpMem" as "(%Hrinr & %Hsrc & HJmpRes)".
+    case_decide as Hdec ; cycle 1.
+    { iDestruct "HJmpRes" as "->".
+      iSplitR. by rewrite lookup_insert.
+      iPureIntro ; intros ? ? Hnz.
+      exists p,b,e,a.
+      split; auto.
+      apply not_and_r in Hdec as [Hcontra|Hcontra]; simplify_eq; cycle 1.
+      apply not_and_r in Hcontra as [Hcontra|Hcontra]; simplify_eq.
+      apply Is_true_true_1 in Hnz.
+      done.
+      by destruct (decide (reg_allows_IE_jmp regs dst p b e a)).
+    }
+    destruct Hdec as (Hdec & _ & Hnz).
+    assert (a <> (a^+1)%a)
+    by (inversion Hdec as (_ & _ & Hwb%withinBounds_true_iff & _); solve_addr).
+    case_decide as Ha; simplify_eq.
+    { iDestruct "HJmpRes" as (w2) "[%Hmem _]" ; subst.
+      iSplitL; iPureIntro.
+      by simplify_map_eq.
+      intros ? ? ?. exists p,b,e,a.
+      split;auto.
+      simplify_eq.
+      case_decide; auto.
+      inversion Hdec.
+      exists pc_w, w2.
+      by split ; simplify_map_eq.
+    }
+    case_decide as Ha'; simplify_eq.
+    { iDestruct "HJmpRes" as (w1) "[%Hmem _]" ; subst.
+      iSplitL; iPureIntro.
+      by simplify_map_eq.
+      intros ? ? ?. exists p,b,e,a.
+      split;auto.
+      simplify_eq.
+      case_decide; auto.
+      inversion Hdec.
+      exists w1, pc_w.
+      by split ; simplify_map_eq.
+    }
+
+    iDestruct "HJmpRes" as (w1 w2) "[%Hmem _]" ; subst.
+    iSplitL; iPureIntro.
+    by simplify_map_eq.
+    intros ? ? ?. exists p,b,e,a.
+    split;auto.
+    simplify_eq.
+    case_decide; auto.
+    exists w1, w2.
+    by split ; simplify_map_eq.
+  Qed.
+
+  Lemma reg_allows_IE_jmp_same
+    (regs : Reg) (r : RegName)
+    (p p' : Perm) (b b' e e' a a' : Addr):
+    reg_allows_IE_jmp regs r p b e a ->
+    regs !! r = Some (WCap p' b' e' a') ->
+    (p = p' /\ b = b' /\ e = e' /\ a = a').
+  Proof.
+    intros HallowJmp Hregs.
+    destruct HallowJmp as (Hregs'&->&_).
+    by rewrite Hregs' in Hregs; simplify_eq.
+  Qed.
+
+  Lemma jnz_case (regs : leibnizO Reg) (p : Perm)
+        (b e a : Addr) (widc w : Word) (dst src : RegName) (P : D):
+    ftlr_instr regs p b e a widc w (Jnz dst src) P.
   Proof.
     intros Hp Hsome i Hbae Hi.
-    iIntros "#IH #Hinv #Hinva #Hreg #Hread Hown Ha HP Hcls HPC Hmap".
-    rewrite delete_insert_delete.
-    iDestruct ((big_sepM_delete _ _ PC) with "[HPC Hmap]") as "Hmap /=";
-      [apply lookup_insert|rewrite delete_insert_delete;iFrame|]. simpl.
-    iApply (wp_Jnz with "[$Ha $Hmap]"); eauto.
-    { simplify_map_eq; auto. }
+    iIntros
+      "#IH #Hinv_pc #Hinv_idc #Hinva #Hreg #[Hread _] Hown Ha HP Hcls HPC HIDC Hmap".
+    iInsertList "Hmap" [idc;PC].
+
+    (* To read out PC's name later, and needed when calling wp_load *)
+    assert(∀ x : RegName, is_Some (<[PC:=WCap p b e a]> (<[idc:=widc]> regs) !! x)) as Hsome'.
+    {
+      intros. destruct (decide (x = PC)).
+      rewrite e0 lookup_insert; unfold is_Some. by eexists.
+      destruct (decide (x = idc)).
+      rewrite lookup_insert_ne; auto.
+      rewrite e0 lookup_insert; unfold is_Some. by eexists.
+      by rewrite! lookup_insert_ne.
+    }
+
+    (* Initializing the names for the values of Hsrc now, to instantiate the existentials in step 1 *)
+    assert (∃ p0 b0 e0 a0, read_reg_inr (<[PC:=WCap p b e a]> (<[idc:=widc]> regs)) dst p0 b0 e0 a0)
+      as [p0 [b0 [e0 [a0 HVdst] ] ] ].
+    {
+      specialize Hsome' with dst as Hdst.
+      destruct Hdst as [wdst Hsomedst].
+      unfold read_reg_inr. rewrite Hsomedst.
+      destruct wdst as [|[ p0 b0 e0 a0|] | ]; try done.
+      by repeat eexists.
+    }
+
+    assert (exists wsrc, (<[PC:=WCap p b e a]> (<[idc:=widc]> regs)) !! src = Some wsrc) as [wsrc HVsrc].
+    {
+      specialize Hsome' with src as Hsrc.
+      destruct Hsrc as [wsrc Hsomesrc].
+      by eexists.
+    }
+
+    (* Step 1: open the region, if necessary, and store all the resources
+       obtained from the region in allow_IE_res *)
+    iDestruct (create_jnz_res with "Hreg Hinv_idc") as (P1 P2) "HJmpRes"; eauto.
+    { destruct Hp ; destruct p ; auto. }
+
+    (* Step2: derive the concrete map of memory we need, and any spatial
+       predicates holding over it *)
+    iMod (jnz_res_implies_mem_map with "HJmpRes Ha") as (mem) "[HJmpMem HJmpRest]".
+
+    (* Step 3:  derive the non-spatial conditions over the memory map*)
+    iDestruct (mem_map_implies_pure_conds with "HJmpMem") as
+      %(HReadPC & HAJmpMem); auto.
+
+    (* Step 3.5:  derive the non-spatial conditions over the registers *)
+    iAssert (⌜allow_jnz_rmap_or_true dst src
+               (<[PC:=WCap p b e a]> (<[idc:=widc]> regs))⌝)%I as "%HAJmpReg".
+    { rewrite /allow_jnz_rmap_or_true.
+      iIntros (wsrc0) "%Hsrc0 %Hnz0".
+      iExists p0, b0, e0, a0.
+      iSplit; auto.
+      case_decide as Heq; auto.
+      by iExists widc; simplify_map_eq.
+    }
+
+    iApply (wp_Jnz _ _ _ _ _ _ _ _ (<[PC:=WCap p b e a]> (<[idc:=widc]> regs))
+             with "[Hmap HJmpRest]");eauto.
+    { by simplify_map_eq. }
     { rewrite /subseteq /map_subseteq /set_subseteq_instance. intros rr _.
-      apply elem_of_dom. apply lookup_insert_is_Some'; eauto. }
+      apply elem_of_dom. repeat (rewrite lookup_insert_is_Some'; right); eauto. }
+    { iSplitR "Hmap"; auto. }
+    iNext. iIntros (regs' retv). iDestruct 1 as (HSpec) "[Hmem Hmap]".
+    (* Infer that if P holds at w, then w must be valid (read condition) *)
+    iDestruct ("Hread" with "HP") as "#Hw".
+    rewrite /allow_jnz_res /allow_jnz_mem /allow_jnz_mask_reg /allow_jnz_mask.
 
-    iIntros "!>" (regs' retv). iDestruct 1 as (HSpec) "[Ha Hmap]".
-    destruct HSpec.
-    { iApply wp_pure_step_later; auto.
-      iMod ("Hcls" with "[Ha HP]");[iExists w;iFrame|iModIntro]. iNext.
-      iIntros "_".
-      iApply wp_value; auto. iIntros; discriminate. }
-    { match goal with
-      | H: incrementPC _ = Some _ |- _ => apply incrementPC_Some_inv in H as (p''&b''&e''&a''& ? & HPC & Z & Hregs')
-      end. simplify_map_eq. rewrite insert_insert.
-      iApply wp_pure_step_later; auto. iMod ("Hcls" with "[Ha HP]");[iExists w;iFrame|iModIntro]. iNext.
-      iIntros "_".
-      iApply ("IH" $! r with "[%] [] [Hmap] [$Hown]"); try iClear "IH"; eauto. iModIntro.
-      rewrite !fixpoint_interp1_eq /=.
-      destruct Hp as [-> | ->];iFrame "Hinv". }
-    { simplify_map_eq. iApply wp_pure_step_later; auto.
-      rewrite !insert_insert.
+    destruct HSpec as
+      [ Hfail
+      | * Hsrc Hdst Hcond Hwb Hwb' Ha Ha' HincrPC (* Success IE true*)
+      | * Hsrc Hdst Hcond HnIE HincrPC (* Success true *)
+      | * Hsrc Hcond HincrPC (* Success false *)
+      ].
+    - (* Fail *)
+      case_decide as HallowJmp; cycle 1.
+      {
+        iModIntro.
+        iDestruct "HJmpMem" as "(_&_&->)". rewrite -memMap_resource_1.
+        iMod ("Hcls" with "[Hmem HP]") as "_";[iExists w;iFrame|iModIntro].
+        iApply wp_pure_step_later; auto.
+        iNext; iIntros "_".
+        iApply wp_value; auto; iIntros; discriminate.
+      }
+      iDestruct "HJmpMem" as "(_&_&H)".
+      destruct HallowJmp as (HallowJmp & _ & Hnz).
+      assert ((a0 ^+ 1)%a ≠ a0) as Ha0eq
+          by (destruct HallowJmp as (_ & _ & Hwb%withinBounds_true_iff & _); solve_addr).
 
-      iMod ("Hcls" with "[HP Ha]");[iExists w;iFrame|iModIntro].
+      (* TODO duplicated proof... could be better *)
+      destruct (decide (a = a0)) as [Ha|Ha]; simplify_map_eq.
+      { (* a = a0 *)
+        iDestruct "H" as (w2) "(->&Hres)". rewrite /region_open_resources'.
+        rewrite memMap_resource_2ne; auto.
+        iDestruct "Hmem" as "(Ha0' & Ha0)".
+        iDestruct "Hres" as "(HP2 & _ & Hcls')".
+        rewrite /allow_jnz_mask.
+        case_decide as H'; simplify_eq.
+        iMod ("Hcls'" with "[HP2 Ha0']") as "_"
+        ; [iNext ; iExists w2; iFrame|iModIntro].
+        iMod ("Hcls" with "[Ha0 HP]") as "_";[iExists w;iFrame|iModIntro].
+        iApply wp_pure_step_later; auto.
+        iNext; iIntros "_".
+        iApply wp_value; auto; iIntros; discriminate.
+      }
+      (* a <> a0 *)
+      destruct (decide (a = (a0 ^+1)%a)) as [Ha'|Ha']; simplify_map_eq.
+      { (* a = a0+1 *)
+        iDestruct "H" as (w1) "(->&Hres)". rewrite /region_open_resources.
+        rewrite memMap_resource_2ne; auto.
+        iDestruct "Hmem" as "(Ha0 & Ha0')".
+        iDestruct "Hres" as "(HP1 & _ & Hcls')".
+        rewrite /allow_jnz_mask.
+        case_decide as H'; simplify_eq; clear H'.
+        case_decide as H'; simplify_eq.
+        iMod ("Hcls'" with "[HP1 Ha0]") as "_"
+        ; [iNext ; iExists w1; iFrame|iModIntro].
+        iMod ("Hcls" with "[Ha0' HP]") as "_";[iExists w;iFrame|iModIntro].
+        iApply wp_pure_step_later; auto.
+        iNext; iIntros "_".
+        iApply wp_value; auto; iIntros; discriminate.
+      }
 
+      (* a <> a0+1 *)
+      iDestruct "H" as (w1 w2) "(->&Hres)". rewrite /region_open_resources2.
+      rewrite memMap_resource_3ne; auto.
+      iDestruct "Hmem" as "(Ha0' & Ha0 & Ha)".
+      iDestruct "Hres" as "(HP1 & HP2 & _& _ & Hcls')".
+      rewrite /allow_jnz_mask.
+      case_decide as H'; simplify_eq ; clear H'.
+      case_decide as H'; simplify_eq ; clear H'.
+      iMod ("Hcls'" with "[HP1 HP2 Ha0 Ha0']") as "_"
+      ; [iNext ; iExists w1, w2; iFrame|iModIntro].
+      iMod ("Hcls" with "[Ha HP]") as "_";[iExists w;iFrame|iModIntro].
+      iApply wp_pure_step_later; auto.
+      iNext; iIntros "_".
+      iApply wp_value; auto; iIntros; discriminate.
+
+
+    - (* Success IE true*)
+      rewrite insert_insert insert_commute //= insert_insert in HincrPC; subst regs'.
+      case_decide as HallowJmp.
+      2: { (* contradiction *)
+        rewrite /reg_allows_IE_jmp in HallowJmp.
+        rewrite /read_reg_inr in HVdst.
+        rewrite Hdst in HVdst; simplify_eq.
+        rewrite Hsrc in HVsrc; simplify_eq.
+        repeat (apply not_and_r in HallowJmp as [HallowJmp|HallowJmp]; simplify_eq).
+      }
+      destruct HallowJmp as (HallowJmp & _ & Hnz).
+      assert (PC <> dst) as Hdst'
+          by (destruct (decide (PC = dst)); auto; simplify_map_eq; by destruct Hp).
+      assert (p0 = IE /\ b0 = b1 /\ e0 = e1 /\ a0 = a1) as (-> & -> & -> & ->)
+          by (by eapply reg_allows_IE_jmp_same)
+      ; simplify_map_eq.
+      assert ((a1 ^+ 1)%a ≠ a1) as Haeq by (apply withinBounds_true_iff in Hwb ; solve_addr).
+      assert (withinBounds b1 e1 a1 ∧ withinBounds b1 e1 (a1 ^+ 1)%a) as Hbounds
+          by (by split ; apply Is_true_true_2).
+
+      iDestruct "HJmpMem" as "(_& %H' & HJmpMem)"; simplify_eq.
+      iDestruct "HJmpRes" as "(_& _ & Hexec &HJmpRes)".
+      case_decide as Ha0; simplify_eq.
+      { (* a = a0 *)
+
+        (* NOTE he next PC is an integer. Thus, it's always safe to execute an integer.
+           I can probably prove this case without further modification in the definition
+           of the LR *)
+
+        iDestruct "HJmpMem" as (w2) "(->& HP2& %Hpers2& Hcls')".
+        iDestruct "HP2" as "#HP2".
+        rewrite /allow_jnz_mask.
+        case_decide ; simplify_eq.
+        rewrite memMap_resource_2ne; auto.
+        simplify_map_eq.
+
+        iDestruct "Hmem" as  "[Ha0' Ha0]".
+        iMod ("Hcls'" with "[HP2 Ha0']") as "_"; [iNext;iExists widc0;iFrame "∗ #"|iModIntro].
+        iMod ("Hcls" with "[HP Ha0]") as "_"; [iNext;iExists wpc;iFrame|iModIntro].
+        iClear "HJmpRes".
+        iApply wp_pure_step_later; auto.
+        iNext ; iIntros "_".
+        destruct wpc; cbn in Hi; try done.
+        iExtract "Hmap" PC as "HPC".
+
+        (* TODO extract as a lemma ? that if (PC = WInt z), then safe to execute.
+           It is the second time that it's used (cf. fundamental.v) *)
+        iApply (wp_bind (fill [SeqCtx])); iSimpl.
+        iApply (wp_notCorrectPC with "HPC").
+        intro Hcontra; inversion Hcontra.
+        iNext; iIntros "HPC"; iSimpl.
+        iApply wp_pure_step_later; [ exact I |].
+        iIntros "!> _".
+        iApply wp_value; iIntros "%"; done.
+      }
+
+      (* a ≠ a0 *)
+      case_decide as Ha0'; simplify_eq.
+      { (* a = a0+1 *)
+
+        iDestruct "HJmpMem" as (w1) "(->& HP1& %Hpers1& Hcls')".
+        iDestruct "HP1" as "#HP1".
+        rewrite /allow_jnz_mask.
+        case_decide ; simplify_eq.
+        case_decide ; simplify_eq.
+        rewrite memMap_resource_2ne; auto.
+        simplify_map_eq.
+
+        iDestruct "Hmem" as  "[Ha0' Ha0]".
+        iMod ("Hcls'" with "[HP1 Ha0']") as "_"; [iNext;iExists wpc;iFrame "∗ #"|iModIntro].
+        iMod ("Hcls" with "[HP Ha0]") as "_"; [iNext;iExists widc0;iFrame|iModIntro].
+        iClear "HJmpRes".
+        iApply wp_pure_step_later; auto.
+        iNext ; iIntros "_".
+
+        iApply ("Hexec" $! _ widc0) ; iFrame "∗ #".
+        iRight; destruct widc0; cbn in Hi; try done.
+
+        rewrite insert_commute //=.
+        repeat (iSplit ; try done).
+      }
+
+      (* a ≠ a0+1 *)
+      iDestruct "HJmpMem" as (w1 w2) "(->& HP1& HP2& %Hpers1& %Hpers2& Hcls')".
+      rewrite /region_open_resources2.
+      iDestruct "HP1" as "#HP1"; iDestruct "HP2" as "#HP2".
+      rewrite /allow_jnz_mask; case_decide ; simplify_eq; case_decide ; simplify_eq.
+      rewrite memMap_resource_3ne; auto.
+      simplify_map_eq.
+
+      iDestruct "Hmem" as  "(Ha0' & Ha0 & Ha)".
+      iMod ("Hcls'" with "[HP1 HP2 Ha0' Ha0]") as "_"; [iNext;iExists wpc,widc0;iFrame "∗ #"|iModIntro].
+      iMod ("Hcls" with "[HP Ha]") as "_"; [iNext;iExists w;iFrame|iModIntro].
+      iClear "HJmpRes".
+      iApply wp_pure_step_later; auto.
+      iNext; iIntros "_".
+
+      iApply "Hexec" ; iFrame "∗ #".
+      rewrite insert_commute //=.
+      repeat (iSplit ; try done).
+
+    - (* Success true *)
+      rewrite insert_insert in HincrPC; subst regs'.
+      case_decide as HallowJmp.
+      { (* contradiction *)
+        rewrite /reg_allows_IE_jmp in HallowJmp.
+        destruct HallowJmp as ((Hregs0 & -> & Hwb & Hwb') & _ & _).
+        simplify_eq.
+      }
+      iModIntro.
+      iDestruct "HJmpMem" as "(_&_&->)". rewrite -memMap_resource_1.
+      iMod ("Hcls" with "[Hmem HP]") as "_";[iExists w;iFrame|iModIntro].
+      iApply wp_pure_step_later; auto.
+
+      set (regs' := <[PC:=updatePcPerm w0]> (<[idc:=widc]> regs)).
       (* Needed because IH disallows non-capability values *)
       destruct w' as [ | [p' b' e' a' | ] | ]; cycle 1.
       {
         rewrite /updatePcPerm.
-        iAssert (fixpoint interp1 (WCap p' b' e' a')) as "HECap".
-        { destruct (decide (r1 = PC)) as [-> | Hne]. by simplify_map_eq.
-          rewrite lookup_insert_ne // in H1.
-          unshelve iDestruct ("Hreg" $! r1 _ _ H1) as "HPCv"; auto.
+        set (pc_p' := if decide (p' = E) then RX else p').
+
+        destruct (decide (p' = E)); simplify_map_eq.
+        (* Special case if p' is E *)
+        - (* p' = E *)
+          iAssert (interp (WCap E b' e' a')) as "Hinterp".
+          {
+          assert ( dst <> PC ).
+          { destruct (decide (dst = PC)) ; simplify_map_eq ; destruct Hp; auto. }
+          simplify_map_eq.
+          destruct (decide (dst = idc)) ; simplify_map_eq; auto.
+          iApply "Hreg"; auto.
+          }
+          rewrite (fixpoint_interp1_eq (WCap E _ _ _)) //=.
+          rewrite (insert_commute _ PC _ (WCap RX _ _ _)) //=.
+          iDestruct ("Hinterp" with "[$Hinv_idc] [$Hmap $Hown]") as "Hcont"; auto.
+        - (* p' ≠ E *)
+        iNext ; iIntros "_".
+        iApply ("IH" $! regs' pc_p' with "[%] [] [Hmap] [$Hown]"); subst regs'.
+        { intro; cbn; by repeat (rewrite lookup_insert_is_Some'; right). }
+        { iIntros (ri v Hri Hri' Hvs).
+          simplify_map_eq.
+          iApply "Hreg"; auto.
         }
+        { rewrite
+            insert_insert
+              (insert_commute _ idc) //=
+              insert_insert.
+          subst pc_p'; simplify_eq.
+          by destruct p'.
+        }
+        { iModIntro.
+          subst pc_p'.
+          iClear "HJmpRes IH Hread".
+          clear Hsome' HVdst HAJmpMem HAJmpReg.
 
-        (* Special case for E-values*)
-        destruct (decide (p' = E)) as [-> | HneE].
-        - iClear "Hinv".
-          rewrite fixpoint_interp1_eq; simpl.
-          iDestruct ("HECap" with "[$Hmap $Hown]") as "Hcont"; auto.
-        - iAssert ([∗ map] k↦y ∈ <[PC:= WCap p' b' e' a']> r, k ↦ᵣ y)%I  with "[Hmap]" as "Hmap".
-          { destruct p'; auto. congruence. }
-          iNext; iIntros "_".
-
-          iApply ("IH" $! (<[PC:=WCap p' b' e' a']> r) with "[%] [] [Hmap] [$Hown]").
-          { cbn. intros. by repeat (rewrite lookup_insert_is_Some'; right). }
-          { iIntros (ri v Hri Hvs).
-            rewrite lookup_insert_ne in Hvs; auto.
-              unshelve iSpecialize ("Hreg" $! ri _ _ Hvs); eauto. }
-          { rewrite insert_insert. iApply "Hmap". }
-          auto.
+          destruct (decide (dst = PC)); simplify_map_eq; auto.
+          destruct (decide (dst = idc)); simplify_map_eq; auto.
+          iApply "Hreg" ; auto.
+        }
+        { iFrame "Hinv_idc". }
       }
-     (* Non-capability cases *)
 
-      all: iNext; iIntros "_".
-     all: iDestruct ((big_sepM_delete _ _ PC) with "Hmap") as "[HPC Hmap] /=";
-      [apply lookup_insert|]; simpl.
-     all: rewrite /updatePcPerm; iApply (wp_bind (fill [SeqCtx]));
+      all: iNext ; iIntros "_".
+      all: iExtract "Hmap" PC as "HPC".
+      all: rewrite /updatePcPerm; iApply (wp_bind (fill [SeqCtx]));
         iApply (wp_notCorrectPC with "HPC"); [intros HFalse; inversion HFalse| ].
-     all: repeat iNext; iIntros "HPC /=".
-     all: iApply wp_pure_step_later; auto.
-     all: iNext; iIntros "_".
-     all: iApply wp_value.
-     all: iIntros.
-     all: discriminate.
-     }
-Qed.
+      all: repeat iNext; iIntros "HPC /=".
+      all: iApply wp_pure_step_later; auto.
+      all: iNext; iIntros "_".
+      all: iApply wp_value;iIntros; discriminate.
+
+    - (* Success IE false *)
+      apply incrementPC_Some_inv in HincrPC as (p''&b''&e''&a''& ? & HPC & Z & Hregs') .
+      rewrite insert_insert in Hregs'; subst regs'.
+      simplify_map_eq.
+
+      case_decide as Heq; simplify_eq.
+      { (* contradiction *)
+        exfalso.
+        destruct Heq as (_& H' & Hnz) ; simplify_eq.
+        congruence.
+      }
+      iModIntro.
+      iDestruct "HJmpMem" as "(_& %H' & ->)"; simplify_eq. rewrite -memMap_resource_1.
+      iMod ("Hcls" with "[Hmem HP]") as "_";[iExists w;iFrame|iModIntro].
+      iApply wp_pure_step_later; auto.
+
+      set (regs' := <[PC:=WCap p'' b'' e'' x]> (<[idc:=widc]> regs)).
+      simplify_map_eq.
+
+      iNext ; iIntros "_".
+      iApply ("IH" $! regs' p'' with "[%] [] [Hmap] [$Hown]"); subst regs'.
+      { intro; cbn; by repeat (rewrite lookup_insert_is_Some'; right). }
+      { iIntros (ri v Hri Hri' Hvs).
+        simplify_map_eq.
+        iApply "Hreg"; auto.
+      }
+      { rewrite
+          insert_insert
+            (insert_commute _ idc) //=
+            insert_insert.
+        iFrame.
+      }
+      { iModIntro.
+        iClear "HJmpRes IH Hread".
+        rewrite !fixpoint_interp1_eq //=; destruct Hp as [-> | ->] ;iFrame "Hinv_pc".
+      }
+      { iFrame "Hinv_idc". }
+  Qed.
 
 End fundamental.
